theories/RTac/Open.v
@@ -20,48 +20,75 @@ Section parameterized.
   Variable Subst_subst : Subst subst expr.
   Variable SubstOk_subst : @SubstOk _ _ _ _ Expr_expr Subst_subst.
 
-  Inductive Ctx :=
-  | CTop
-  | CAll : typ -> Ctx -> Ctx
-  | CEx  : typ -> Ctx -> Ctx
-  | CHyp : expr -> Ctx -> Ctx.
-
-  Fixpoint openGoal' (g : Goal typ expr subst) (ctx : Ctx)
-  : Ctx * subst * option expr :=
+  Fixpoint openGoal' (g : Goal typ expr subst) (ctx : Ctx typ expr)
+  : Ctx typ expr * subst * option expr :=
     match g with
-      | GGoal s e => (ctx,s,e)
-      | GAlls t g => openGoal' g (CAll t ctx)
-      | GExs  t g => openGoal' g (CEx  t ctx)
-      | GHyps h g => openGoal' g (CHyp h ctx)
+      | GGoal s e => (ctx,s,Some e)
+      | GSolved s => (ctx,s,None)
+      | GAll t g => openGoal' g (CAll ctx t)
+      | GEx  t g => openGoal' g (CEx  ctx t)
+      | GHyp h g => openGoal' g (CHyp ctx h)
     end.
 
   Definition openGoal g := @openGoal' g CTop.
 
-  Fixpoint closeGoal (ctx : Ctx) (g : Goal typ expr subst)
+  Fixpoint closeGoal (ctx : Ctx typ expr) (g : Goal typ expr subst)
   : Goal typ expr subst :=
     match ctx with
       | CTop => g
-      | CAll t c => closeGoal c (GAlls t g)
-      | CEx t c => closeGoal c (GExs t g)
-      | CHyp t c => closeGoal c (GHyps t g)
+      | CAll c t => closeGoal c (GAll t g)
+      | CEx  c t => closeGoal c (GEx t g)
+      | CHyp c h => closeGoal c (GHyp h g)
     end.
 
-  Fixpoint getEnvs' (ctx : Ctx) (tus tvs : tenv typ) : tenv typ * tenv typ :=
+  Fixpoint getEnvs' (ctx : Ctx typ expr) (tus tvs : tenv typ)
+  : tenv typ * tenv typ :=
     match ctx with
       | CTop => (tus,tvs)
-      | CAll t ctx' => getEnvs' ctx' tus (t :: tvs)
-      | CEx  t ctx' => getEnvs' ctx' (t :: tus) tvs
-      | CHyp _ ctx' => getEnvs' ctx' tus tvs
+      | CAll ctx' t => getEnvs' ctx' tus (t :: tvs)
+      | CEx  ctx' t => getEnvs' ctx' (t :: tus) tvs
+      | CHyp ctx' _ => getEnvs' ctx' tus tvs
     end.
 
-  Definition getEnvs (ctx : Ctx) : tenv typ * tenv typ :=
+  Definition getEnvs (ctx : Ctx typ expr) : tenv typ * tenv typ :=
     let (x,y) := getEnvs' ctx nil nil in
     (x, y).
+
+  Fixpoint countVars' (ctx : Ctx typ expr) acc : nat :=
+    match ctx with
+      | CTop => acc
+      | CAll ctx' t => countVars' ctx' (S acc)
+      | CEx  ctx' _
+      | CHyp ctx' _ => countVars' ctx' acc
+    end.
+
+  Fixpoint countUVars' (ctx : Ctx typ expr) acc : nat :=
+    match ctx with
+      | CTop => acc
+      | CEx  ctx' t => countUVars' ctx' (S acc)
+      | CAll ctx' _
+      | CHyp ctx' _ => countUVars' ctx' acc
+    end.
+
+
+  Definition countVars ctx := countVars' ctx 0.
+  Definition countUVars ctx := countUVars' ctx 0.
 
 (*
   Eval compute in fun t u v a b =>
       let '(x,_,_) := openGoal (GAlls t (GAlls u (GAlls v (GGoal a b)))) in
       getEnvs x.
 *)
+
+
+(**
+  Definition finish : rtac typ expr subst :=
+    fun g =>
+      let '(ctx,s,gl) := openGoal g in
+      let (tus,tvs) := getEnvs ctx in
+      let (ctx',s) := reduceGoal ctx s (length tus) (length tvs) in
+      Some (closeGoal ctx' (GGoal s None)).
+**)
+
 
 End parameterized.
