theories/RTac/RTac.v
@@ -8,6 +8,7 @@ Require Export MirrorCore.RTac.Repeat.
 Require Export MirrorCore.RTac.Assumption.
 Require Export MirrorCore.RTac.RunSTac.
 Require Export MirrorCore.RTac.Intro.
+(*
 Require Export MirrorCore.RTac.Apply.
 Require Export MirrorCore.RTac.EApply.
 
@@ -15,3 +16,4 @@ Require Export MirrorCore.RTac.AtGoal.
 
 Require Export MirrorCore.RTac.Continuation.
 Require Export MirrorCore.RTac.ApplyToAll.
+*)
